ulib/FStar.SizeT.fsti
@@ -23,22 +23,26 @@ val size_v_inj (x1 x2: t) : Lemma
 /// Any value that fits in a uint_16 can be cast directly to t
 /// Any value that might not fit in a uint_16 needs to be checked,
 /// we will add a static_assert during extraction
+val uint_to_t (x: nat) : Pure t
+  (requires (fits x))
+  (ensures (fun y -> v y == x))
+
+noextract inline_for_extraction
 val mk (x: U16.t) : Pure t
   (requires True)
   (ensures (fun y -> v y == U16.v x))
 
+noextract inline_for_extraction
 val mk_checked (x: U64.t) : Pure t
   (requires True)
   (ensures (fun y -> v y == U64.v x))
 
-val int_to_t (x: nat) : Ghost t
-  (requires (fits x))
-  (ensures (fun y -> v y == x))
-
-val fits_le (x y: nat) : Lemma
+val fits_lte (x y: nat) : Lemma
   (requires (x <= y /\ fits y))
   (ensures (fits x))
   [SMTPat (fits x); SMTPat (fits y)]
+
+(** Non-overflowing arithmetic operations *)
 
 val add (x y: t) : Pure t
   (requires (fits (v x + v y)))
@@ -52,10 +56,40 @@ val mul (x y: t) : Pure t
   (requires (fits (v x * v y)))
   (ensures (fun z -> v z == v x * v y))
 
-val le (x y: t) : Pure bool
+(** Greater than *)
+val gt (x y:t) : Pure bool
+  (requires True)
+  (ensures (fun z -> z == (v x > v y)))
+
+(** Greater than or equal *)
+val gte (x y:t) : Pure bool
+  (requires True)
+  (ensures (fun z -> z == (v x >= v y)))
+
+(** Less than *)
+val lt (x y:t) : Pure bool
+  (requires True)
+  (ensures (fun z -> z == (v x < v y)))
+
+(** Less than or equal *)
+val lte (x y: t) : Pure bool
   (requires True)
   (ensures (fun z -> z == (v x <= v y)))
 
+(** Common constants *)
+
+noextract inline_for_extraction
 let zero : (zero_size: t { v zero_size == 0 }) = mk 0us
 
+noextract inline_for_extraction
 let one : (zero_size: t { v zero_size == 1 }) = mk 1us
+
+(** Infix notations *)
+
+unfold let op_Plus_Hat = add
+unfold let op_Subtraction_Hat = sub
+unfold let op_Star_Hat = mul
+unfold let op_Greater_Hat = gt
+unfold let op_Greater_Equals_Hat = gte
+unfold let op_Less_Hat = lt
+unfold let op_Less_Equals_Hat = lte
